Add typeclass for blinded values

isa/Value.fst
@@ -6,10 +6,27 @@
 /// on them.
 module Value
 
+class blinded_data_representation (outer:eqtype) = {
+  inner: eqtype;
+  equiv: outer -> outer -> bool;
+  is_blinded: outer -> bool;
+  redact: outer -> inner -> outer;
+  [@@@FStar.Tactics.Typeclasses.no_method]
+  properties: squash (
+    (forall (x y: outer). x = y ==> equiv x y) /\
+    (forall (x y: outer). equiv x y <==> equiv y x) /\
+    (forall (x y z: outer). equiv x y /\ equiv y z ==> equiv x z) /\
+    (forall (x: outer) (d: inner). equiv x (redact x d))
+  )
+}
+
+let (≡) #a {| blinded_data_representation a |} (lhs rhs : a): bool = equiv lhs rhs
+
 /// The ``maybeBlinded`` type represents a type that may be blinded:
 type maybeBlinded (#t:Type) =
    | Clear   : v:t -> maybeBlinded #t (* Represents a non-blinded value *)
    | Blinded : v:t -> maybeBlinded #t (* Represents a blinded value *)
+
 
 /// But since most software is not written with knowledge of blindable values,
 /// we need a way to unwrap the blindable value and get the value inside.
@@ -31,15 +48,15 @@ let unwrap (#t:Type) (mb:maybeBlinded #t): t =
 ///
 /// This means that they must have the same blindedness, and if they aren't
 /// blinded then they must have the same values too:
-val equiv (#t:eqtype)
+val equiv1 (#t:eqtype)
     (lhs:maybeBlinded #t)
     (rhs:maybeBlinded #t)
-    : r:prop{r <==> (    (Blinded? lhs /\ Blinded? rhs)
-                      \/ (Clear?   lhs /\ Clear?   rhs  /\ Clear?.v lhs == Clear?.v rhs) )}
+    : r:bool{r <==> (    (Blinded? lhs /\ Blinded? rhs)
+                      \/ (Clear?   lhs /\ Clear?   rhs  /\ Clear?.v lhs = Clear?.v rhs) )}
 
-let equiv lhs rhs
+let equiv1 lhs rhs
     = match lhs, rhs with
-      | Clear x, Clear y -> (x == y)
+      | Clear x, Clear y -> (x = y)
       | Blinded _, Blinded _ -> true
       | _ -> false
 
@@ -48,27 +65,65 @@ let equiv lhs rhs
 ///  - **Reflexivity**
 let equal_values_are_equivalent (t:eqtype) (lhs rhs:maybeBlinded #t):
   Lemma (requires lhs = rhs)
-        (ensures equiv lhs rhs) =
+        (ensures equiv1 lhs rhs) =
   ()
 
 ///  - **Symmetry**
 let equivalence_is_symmetric (t:eqtype) (lhs rhs: maybeBlinded #t):
-    Lemma (requires equiv lhs rhs)
-          (ensures  equiv rhs lhs)
+    Lemma (requires equiv1 lhs rhs)
+          (ensures  equiv1 rhs lhs)
     = ()
 
 ///  - **Transitivity**
 let equivalence_is_transitive (t:eqtype) (lhs mid rhs:maybeBlinded #t):
-    Lemma (requires (equiv lhs mid) /\ (equiv mid rhs))
-          (ensures   equiv lhs rhs)
+    Lemma (requires (equiv1 lhs mid) /\ (equiv1 mid rhs))
+          (ensures   equiv1 lhs rhs)
     = ()
 
 /// Finally, we show that equivalence on non-blinded values is just the
 /// normal equality relation.
 let equivalent_clear_values_are_equal (t:eqtype) (x y:maybeBlinded #t):
-    Lemma (requires Clear? x /\ Clear? y /\ equiv x y)
+    Lemma (requires Clear? x /\ Clear? y /\ equiv1 x y)
           (ensures x = y)
     = ()
+
+/// ---------
+/// Redaction
+/// ---------
+///
+/// Next we define a notion of redaction.  This replaces blinded values
+/// with some fixed blinded value, so that the redaction of a blindable value
+/// is a representative of its equivalence class.
+let redact1 (#t:Type) (x: maybeBlinded #t) (d:t): maybeBlinded #t =
+    match x with
+    | Clear   v -> Clear v
+    | Blinded t -> Blinded d
+
+let _ = assert(forall (t:eqtype) (x y d: t). redact1 (Blinded x) d == redact1 (Blinded y) d)
+
+/// The result is that we obtain an equivalent value to the input that is
+/// independent of all of its sensitive values.
+let values_are_equivalent_to_their_redaction (t:eqtype) (x:maybeBlinded #t) (d:t):
+    Lemma (ensures equiv1 x (redact1 x d))
+    = ()
+
+/// Since the redaction of an element is a representative of its equivalence class,
+/// the redaction of two values is equal if and only if they are equivalent.
+let equivalent_values_have_equal_redactions (t:eqtype) (x y:maybeBlinded #t) (d:t):
+    Lemma (ensures equiv1 x y <==> redact1 x d = redact1 y d)
+    = ()
+
+
+instance single_bit_blinding (#t:eqtype) : blinded_data_representation (maybeBlinded #t) = {
+  inner = t;
+  equiv = equiv1;
+  is_blinded = (fun (x: maybeBlinded #t) -> Blinded? x);
+  redact = redact1;
+  properties =  ()
+}
+
+
+
 /// ^^^^^^^^^^^^^^^^^^^^^^^^^^^^^^^^^^^^^^^^
 /// Equivalence of lists of blindable values
 /// ^^^^^^^^^^^^^^^^^^^^^^^^^^^^^^^^^^^^^^^^
@@ -78,21 +133,17 @@ let equivalent_clear_values_are_equal (t:eqtype) (x y:maybeBlinded #t):
 ///
 /// .. fst::
 ///    :name: equiv_list
-val equiv_list (#t:eqtype)
-      (lhs:list (maybeBlinded #t))
-      (rhs:list (maybeBlinded #t))
-      : prop
 
-let rec equiv_list (lhs:list maybeBlinded) (rhs: list maybeBlinded)
+let rec equiv_list #t {| blinded_data_representation t |} (lhs:list t) (rhs: list t): bool
     = match lhs, rhs with
        | Nil,      Nil      -> true
        | Nil,      Cons _ _ -> false
        | Cons _ _, Nil      -> false
-       | lh :: lt,  rh :: rt  -> (equiv lh rh) /\ (equiv_list lt rt)
+       | lh :: lt,  rh :: rt  -> (lh ≡ rh) && (equiv_list lt rt)
 
 
 /// First, we show that equivalent lists must have equal lengths.
-let rec equivalent_lists_have_equal_lengths (#t:eqtype) (l1 l2:list (maybeBlinded #t))
+let rec equivalent_lists_have_equal_lengths #t {| blinded_data_representation t |} (l1 l2:list t)
   : Lemma (requires equiv_list l1 l2)
           (ensures FStar.List.length l1 = FStar.List.length l2)
   = match l1, l2 with
@@ -102,25 +153,25 @@ let rec equivalent_lists_have_equal_lengths (#t:eqtype) (l1 l2:list (maybeBlinde
 /// Then we show that list equivalence is an equivalence relation:
 ///
 ///  - **Reflexivity**
-let rec equal_lists_are_equivalent (t:eqtype) (lhs rhs:list(maybeBlinded #t)):
+let rec equal_lists_are_equivalent t {| blinded_data_representation t |} (lhs rhs:list t):
     Lemma (requires lhs = rhs)
           (ensures equiv_list lhs rhs) =
     match lhs, rhs with
       | Nil, Nil -> ()
-      | hl :: tl, hr :: tr -> (equal_values_are_equivalent t hl hr;
-                            equal_lists_are_equivalent t tl tr)
+      | hl :: tl, hr :: tr -> (//equal_values_are_equivalent #t hl hr;
+                             equal_lists_are_equivalent t tl tr)
 
 ///  - **Symmetry**
-let rec list_equivalence_is_symmetric (t:eqtype) (lhs rhs: list(maybeBlinded #t)):
-    Lemma (requires equiv_list lhs rhs)
-          (ensures   equiv_list rhs lhs)
-          [SMTPat (equiv_list lhs rhs)]
+let rec list_equivalence_is_symmetric t {| blinded_data_representation t |} (lhs rhs: list t):
+    Lemma (requires equiv_list #t lhs rhs)
+          (ensures  equiv_list #t rhs lhs)
+          [SMTPat (equiv_list #t lhs rhs)]
     = match lhs, rhs  with
       | hl :: tl, hr :: tr -> list_equivalence_is_symmetric t tl tr
       | _ -> ()
 
 ///  - **Transitivity**
-let rec list_equivalence_is_transitive (t:eqtype) (lhs mid rhs: list(maybeBlinded #t)):
+let rec list_equivalence_is_transitive t {| blinded_data_representation t |} (lhs mid rhs: list t):
     Lemma (requires (equiv_list lhs mid) /\ (equiv_list mid rhs))
           (ensures   equiv_list lhs rhs)
     = match lhs, mid, rhs  with
@@ -130,17 +181,17 @@ let rec list_equivalence_is_transitive (t:eqtype) (lhs mid rhs: list(maybeBlinde
 
 /// For convenience, we define our own ``nth`` function to extract the value at
 /// a particular index.
-let nth (#t:eqtype) (m:list (maybeBlinded #t)) (n:nat{n < FStar.List.length m}): maybeBlinded #t =
+let nth  t {| blinded_data_representation t |} (m: list t) (n:nat{n < FStar.List.length m}): t =
   FStar.List.Tot.index m n
 
 /// Then, we prove that extracting values from equivalent lists yields
 /// equivalent values:
-let rec equivalent_lists_have_equivalent_values (t:eqtype)
-                                                (a b: list (maybeBlinded #t))
+let rec equivalent_lists_have_equivalent_values t {| blinded_data_representation t |}
+                                                (a b: list t)
                                                 (n: nat{n < FStar.List.length a &&
                                                       n < FStar.List.length b}):
     Lemma (requires equiv_list a b)
-          (ensures equiv (FStar.List.Tot.index a n) (FStar.List.Tot.index b n))
+          (ensures (FStar.List.Tot.index a n) ≡ (FStar.List.Tot.index b n))
     = match n, a, b  with
       | 0, _, _ -> ()
       | _, hl :: tl, hr :: tr -> equivalent_lists_have_equivalent_values _ tl tr (n - 1)
@@ -148,47 +199,28 @@ let rec equivalent_lists_have_equivalent_values (t:eqtype)
 
 /// We also show all lists of blinded values are equivalent to one another, so
 /// long as they have the same length.
-let rec all_values_are_blinded (t:eqtype) (l: list (maybeBlinded #t)) =
+let rec all_values_are_blinded #t {| blinded_data_representation t |} (l: list t) =
   match l with
-    | hd :: tl -> if Clear? hd then false else all_values_are_blinded t tl
+    | hd :: tl -> if not (is_blinded hd) then false else all_values_are_blinded tl
     | _ -> true
 
-let rec lists_of_blinded_values_of_equal_length_are_equivalent (t:eqtype) (a b: list (maybeBlinded #t)):
+let rec lists_of_blinded_values_of_equal_length_are_equivalent (#t:eqtype) (a b: list (maybeBlinded #t)):
   Lemma (requires (FStar.List.length a = FStar.List.length b)
-                /\ (all_values_are_blinded t a) /\ (all_values_are_blinded t b))
+                /\ (all_values_are_blinded a) /\ (all_values_are_blinded b))
         (ensures equiv_list a b) =
   match a, b with
     | h1 :: t1, h2 :: t2 -> (
-         lists_of_blinded_values_of_equal_length_are_equivalent t t1 t2
+         assert(is_blinded h1 /\ is_blinded h2);
+         assert(h1 ≡ h2);
+         lists_of_blinded_values_of_equal_length_are_equivalent #t t1 t2
       )
     | _ -> ()
 
+let rec any_value_is_blinded #t {| blinded_data_representation t |} (l: list t) =
+  match l with
+    | hd :: tl -> if is_blinded hd then true else any_value_is_blinded #t tl
+    | _ -> false
 
-/// ---------
-/// Redaction
-/// ---------
-///
-/// Next we define a notion of redaction.  This replaces blinded values
-/// with some fixed blinded value, so that the redaction of a blindable value
-/// is a representative of its equivalence class.
-let redact (#t:Type) (x: maybeBlinded #t) (d:t): maybeBlinded #t =
-    match x with
-    | Clear   v -> Clear v
-    | Blinded t -> Blinded d
-
-let _ = assert(forall (t:eqtype) (x y d: t). redact (Blinded x) d == redact (Blinded y) d)
-
-/// The result is that we obtain an equivalent value to the input that is
-/// independent of all of its sensitive values.
-let values_are_equivalent_to_their_redaction (t:eqtype) (x:maybeBlinded #t) (d:t):
-    Lemma (ensures equiv x (redact x d))
-    = ()
-
-/// Since the redaction of an element is a representative of its equivalence class,
-/// the redaction of two values is equal if and only if they are equivalent.
-let equivalent_values_have_equal_redactions (t:eqtype) (x y:maybeBlinded #t) (d:t):
-    Lemma (ensures equiv x y <==> redact x d = redact y d)
-    = ()
 
 
 /// We can also define redaction on lists, by redacting each of their elements.
@@ -236,3 +268,27 @@ let rec redacted_lists_have_redacted_values (t:eqtype)
       | 0, _ -> ()
       | _, hl :: tl -> redacted_lists_have_redacted_values _ tl d (n - 1)
       | _ -> ()
+
+
+
+// let props t {| blinded_data_representation t |} : Lemma (ensures (
+//     (forall (x y: list t). x = y ==> equiv_list x y) /\
+//     (forall (x y: list t). equiv_list x y <==> equiv_list y x) /\
+//     (forall (x y z: list t). equiv_list x y /\ equiv_list y z ==> equiv_list x z)
+//   )) =
+//     let lem1 lhs rhs : Lemma (lhs = rhs ==> equiv_list lhs rhs) = FStar.Classical.move_requires (equal_lists_are_equivalent t lhs) rhs in
+//     FStar.Classical.forall_intro_2 lem1;
+//     assert(forall (x y: list t). x = y ==> equiv_list x y); // by (
+//     assert(forall (x y: list t). equiv_list x y <==> equiv_list y x);
+
+//     let lem3 lhs mid rhs : Lemma (equiv_list lhs mid /\ equiv_list mid rhs ==> equiv_list lhs rhs) = FStar.Classical.move_requires (list_equivalence_is_transitive t lhs mid) rhs in
+//     FStar.Classical.forall_intro_3 lem3;
+//     assert(forall (x y z: list t). equiv_list x y /\ equiv_list y z ==> equiv_list x z);
+//     ()
+
+
+// instance list_blinding (#t:eqtype) : blinded_data_representation (list (maybeBlinded #t)) = {
+//   equiv = equiv_list;
+//   is_blinded = (fun x -> (true == all_values_are_blinded t x));
+//   properties = props t
+// }
